TransitionSystem.v
@@ -1,8 +1,9 @@
 From mathcomp Require Import ssreflect ssrfun ssrbool ssrnat seq fintype order.
 From mathcomp Require Import eqtype fingraph path. 
 From event_struct Require Import utilities EventStructure.
+From Coq Require Import ssrsearch Lia.
 
-Section transition_system.
+Section TransitionSystem.
 
 Context {val : eqType}.
 
@@ -12,68 +13,71 @@ Notation cexec_event_struct := (@cexec_event_struct val).
 Notation label := (@label val).
 Notation n := (@n val).
 
-Implicit Types (x : var) (a : val).
+Implicit Types (x : var) (a : val) (es : exec_event_struct).
 
 (* Section with definitions for execution graph with added event *)
 Section adding_event.
 
 (* execution graph in which we want to add l *)
-Variable es : exec_event_struct.
+Context (es : exec_event_struct).
 
 Notation n      := (n es).
 Notation lab    := (lab es).
 Notation fpred  := (fpred es).
 Notation frf    := (frf es).
 
+Inductive add_label :=
+  Add : forall 
+    (l : label),
+    option 'I_n ->
+    (is_read l -> {k : 'I_n | compatible (te_ext lab k) l}) ->
+    add_label.
+
+Variable al : add_label.
+
 (* label of an event which we want to add     *)
-Variable l : label.
+Definition l := let '(Add lb _ _) := al in lb.
+(*Variable l : label.*)
 
- (* predecessor of the new event (if it exists) *)
-Variable op : option 'I_n.
+(* predecessor of the new event (if it exists) *)
+Definition op := let '(Add _ opr _) := al in opr.
+(*Variable op : option 'I_n.*)
 
-(* if event is `R` then we should give `W` from wich we read *)
-Variable ow : is_read l -> {k : 'I_n | compatible (te_ext lab k) l}.
+(* if event is `Read` then we should give `Write` from wich we read *)
+Definition ow : is_read l -> {k : 'I_n | compatible (te_ext lab k) l}.
+  rewrite /l. case: al=> ??. exact. Defined.
+(*Variable ow : is_read l -> {k : 'I_n | compatible (te_ext lab k) l}.*)
 
 Definition add_lab : 'I_n.+1 -> label := 
-  @upd (fun _ => label) n lab l.
+  @upd (fun=> label) n lab l.
 
 Definition add_fpred : forall m : 'I_n.+1, option 'I_m := 
-  @upd (fun m => option 'I_m) n fpred op.
-
-(* auxiliary lemma  *)
-(*Lemma advance_is_read {m : 'I_n} : 
-  compatible (te_ext lab m) (te_ext add_lab n) ->
-  compatible_ext add_lab m n.
-Proof. Admitted.*)
-
-(* auxiliary lemma *)
-(* Lemma is_read_add_lab k neq:  *)
-(*   is_read (add_lab k) -> is_read (lab (decr_ord k neq)). *)
-(* Proof. *)
-(* have->//: add_lab k = lab (decr_ord k neq). case: k neq=> /= m ? neq. *)
-(* case: eqP=> [/neq|?]//. by apply/congr1/ord_inj. *)
-(* Qed. *)
+  @upd (option \o ordinal) n fpred op.
 
 Arguments add_lab : simpl never.
 
-(*Lemma add_lab_is_read {r : 'I_n} : 
-  (is_read \o lab) r <-> (is_read \o add_lab) (inc_ord r).
-Proof. Admitted.*)
-
-Lemma is_read_ext_add_lab {r : 'I_n} : 
+Lemma is_read_add_lab {r : 'I_n} :
   is_read_ext add_lab r -> is_read_ext lab r.
-Proof. by rewrite /add_lab dv_ext_upd. Qed.
+Proof. by rewrite /add_lab ext_upd. Qed.
 
 Lemma add_lab_compatible {w r : nat}
   (_ : compatible_ext lab w r) : compatible_ext add_lab w r.
-Proof. rewrite /add_lab rel_dv_ext //. by case. Qed.
+Proof. rewrite /add_lab rel_ext //. by case. Qed.
 
-Lemma ow_add_lab: is_read_ext add_lab n -> {r : 'I_n | compatible_ext add_lab r n}.
-Proof.
-  have E: (te_ext add_lab n) = l by rewrite dv_ext_upd_n.
-  rewrite /= E => /ow [r]. rewrite -E.
-  exists r. by rewrite /comp2 /add_lab dv_ext_upd.
-Qed.
+Lemma is_read_add_lab_n: is_read_ext add_lab n = is_read l.
+Proof. by rewrite /add_lab ext_upd_n. Qed.
+
+Lemma is_read_add_lab_n_aux: is_read_ext add_lab n -> is_read l.
+Proof. by rewrite is_read_add_lab_n. Qed.
+
+Lemma compatible_add_lab (r : 'I_n) : 
+  compatible (te_ext lab r) l -> compatible_ext add_lab r n.
+Proof. by rewrite /add_lab /comp2 ext_upd ext_upd_n. Qed.
+
+Definition  ow_add_lab (is_r : is_read_ext add_lab n) :
+  {r : 'I_n |compatible_ext add_lab r n} :=
+   let w := ow (is_read_add_lab_n_aux is_r) in
+     @exist _ _ (sval w) (compatible_add_lab _ (sproof w)).
 
 Definition add_frf : forall
   (r : 'I_n.+1)
@@ -86,35 +90,109 @@ Definition add_frf : forall
   let frf' (r : 'I_n) : T r := 
       fun is_r =>
         let fP (w : 'I_r) := @add_lab_compatible w r in
-        sproof_map fP (frf r (is_read_ext_add_lab is_r))
+        sproof_map fP (frf r (is_read_add_lab is_r))
   in
-  @upd T n frf' ow_add_lab.
+  upd frf' ow_add_lab.
+
+Lemma sval_add_frf (e1 : 'I_n.+1) (e2 : 'I_n) p p' : e1 = e2 :> nat ->
+  sval (add_frf e1 p) = sval (frf e2 p') :> nat.
+Proof.
+  case: e1 e2 p p'=> ? L1 [? L2 /= P1 P2] E. case: _ / E P1 P2 L1 L2 => *.
+  rewrite /add_frf upd_lt /=. do ?apply /congr1. exact: eq_irrelevance.
+Qed.
+
+Definition add_event := Pack n.+1 add_lab add_fpred add_frf.
+
+Lemma ofpred_add_event e : ofpred add_event e =
+  if e == n then omap (@nat_of_ord n) op else ofpred es e.
+Proof.
+  rewrite /ofpred. insub_case=> L; insub_case=> ?; try case : ifP; try slia.
+  { move=> ?. apply /congr1. by rewrite /add_fpred upd_lt. }
+  move=> /eqP /esym E. move: E L. case: _ / => ?. 
+  by rewrite /add_fpred upd_ord_max.
+Qed.
+
+Definition owr := 
+  (if is_read l as is_r return (is_read l = is_r -> option nat) then
+    fun pf => some (nat_of_ord (sval (ow pf))) 
+  else fun=> none) erefl.
+
+Lemma sval_oread {e}: 
+  (e == n = false) -> 
+  omap ((@nat_of_ord n) \o sval) (oread es e) =
+  omap ((@nat_of_ord n.+1) \o sval) (oread add_event e).
+Proof.
+  move=> ?. rewrite /oread. insub_case; dcase; (try slia)=> ? L.
+  case R: (is_read_ext lab e).
+  { by rewrite ?insubT /= /add_lab -[e]/(nat_of_ord (ord L)) ext_upd. }
+  by rewrite ?insubF //= /add_lab -[e]/(nat_of_ord (ord L)) ext_upd.
+Qed.
+
+Arguments oread : simpl never.
+
+Lemma ofrf_add_event e: ofrf add_event e = 
+  if e == n then owr else ofrf es e.
+Proof.
+  rewrite /ofrf/=. case: ifP=> [/eqP ->| efn].
+  { rewrite /owr. dcase.
+    { rewrite /oread /=. insub_case=> [? R|]; last slia.
+      rewrite insubT /= ?is_read_add_lab_n // => R'. 
+      rewrite /add_frf upd_ord_max /=. do? apply /congr1. 
+      exact: eq_irrelevance. }
+    rewrite /oread /=. insub_case=> *. 
+    by rewrite insubF // is_read_add_lab_n. }
+  case H: (oread add_event e)=> [[/=]|];
+  move: (H) (sval_oread efn)=>->/=; case H': (oread es e) => //= [[/=]][?].
+  exact /congr1 /sval_add_frf.
+Qed.
+
+(*Lemma ica_add_event e1 e2: 
+  ica add_event e1 e2 = 
+    if (e2 == n) then
+       (omap (@nat_of_ord n) op == some e1) || (owr == some e1)
+    else ica es e1 e2.
+Proof. 
+  rewrite /ica /succ /rf ofrf_add_event ofpred_add_event. by case: ifP. 
+Qed.*)
+
+Lemma ica_add_event e1 e2: 
+  ica add_event e1 e2 =
+  (ica es e1 e2) || 
+  ((e2 == n) && ((omap (@nat_of_ord n) op == some e1) || (owr == some e1))).
+Proof.
+  rewrite /ica /succ /rf ofrf_add_event ofpred_add_event. case: ifP=>/=.
+  { move /eqP->. by rewrite ofpred_n ?ofrf_n. }
+  by rewrite orbF.
+Qed.
+
+Hypothesis consist : consistency es.
+Hypothesis ncf_rf : forall e, owr = some e -> ~~ (cf add_event n e).
+
+Lemma ca_add_event e1 e2: e2 != n -> ca es e1 e2 = ca add_event e1 e2.
+Proof. Admitted.
+
+Lemma cf_add_event e1 e2  (_ : e1 != n) (_ : e2 != n) :
+  cf es e1 e2 = cf add_event e1 e2.
+Proof. Admitted.
+
+Lemma consist_add_event: consistency add_event.
+Proof.
+  rewrite /consistency. apply /forallP=> e1. apply /forallP => e2.
+  apply /implyP=> /eqP. rewrite ofrf_add_event. case: ifP=> [/eqP->/ncf_rf|]//.
+  case: e1 e2=> /= x? [y? /=]. case yEn: (x == n).
+  { move /eqP: yEn=>-> ? /ofrf_le. slia. }
+  move=> E. move /rff_consist: consist => /apply cf. apply /negP=> cf'.
+  apply /cf. rewrite cf_add_event; slia.
+Qed.
 
 End adding_event.
 
-Section add_event_def.
-Variables (e : exec_event_struct) (ipred : option 'I_(n e)).
+Definition tr_add_event es1 es2 := exists al, es2 = add_event es1 al.
 
+Notation "es1 '-->' es2" := (tr_add_event es1 es2) (at level 0).
 
+Definition ltr_add_event es1 al es2 := es2 = add_event es1 al.
 
-(*Inductive add_label := 
-| add_W : tid -> var -> val -> add_label
-| add_R (n : 'I_(n e)) t x a : ocompatible (ext (lab e) n) (some (R t x a)) -> add_label.
+Notation "es1 '--' al '-->' es2" := (ltr_add_event es1 al es2) (at level 0).
 
-Definition add_event (l : add_label) := 
-  match l with
-  | add_W t x a      => Pack 
-                         (n e).+1 
-                         (add_lab (W t x a) e)
-                         (add_pred e ipred) 
-                         (add_rf_None (W t x a) e ipred not_false_is_true)
-  | add_R k t x a RF => Pack
-                         (n e).+1 
-                         (add_lab (R t x a) e)
-                         (add_pred e ipred)
-                         (add_rf_some (R t x a) e ipred k RF)
-  end.*)
-
-End add_event_def.
-
-End transition_system.
+End TransitionSystem.
